%% This is an example first chapter.  You should put chapter/appendix that you
%% write into a separate file, and add a line \include{yourfilename} to
%% main.tex, where `yourfilename.tex' is the name of the chapter/appendix file.
%% You can process specific files by typing their names in at the 
%% \files=
%% prompt when you run the file main.tex through LaTeX.
\chapter{Introduction}
In this thesis I studied a 1-dimensional interacting particle system model called q-TASEP. It's one of the most recently yet classical particle model in this field that has important application in the physical world. For example, the model can be used to study mass transport, traffic flow and queuing behaviour etc. The article is concerned with the asymptotic behavior of the particles and is going to provide an explicit formulat describing the behavior. The approach starts from the duality between the q-TASEP model and another model called q-TAZRP. 

We are going to define the two model, q-TASEP and q-TAZRP in this chapter, and show some calculations of the q-TASEP from elementary approach. After this prove their duality in \textit{Chapter 2}. Then we provide an ansatz explicit formula for the expectation of q-Laplace transform of the probability function describing the position of a particular particle at any time in the future in form of the nested contour integral. In the chapter that follows we work to transform a generating function of the nested contour integral we have obtained into the form of a Fredholm determinant, using two different approaches. Lastly in \textit{Chapter 4} we perform asymptotic analysis to the Fredholm determinant and conclude that the rescaled fluctuation of the particle around the macroscopic follows a GUE Tracy-Widom distribution.

\section{Introduction to q-TASEP}
\label{sec:intro-qtasep}

q-TASEP, short for q-deformed totally asymmetric simple exclusion process, refers to a continuous time, discrete space Markov Process $\vec{x}(t)$ describing the dynamics of the following interacting particle system:

\begin{itemize}
\item Particles denoted by $\{x_1, x_2, x_3, ...\}$ occupy sites of $\mathbb{Z}$ exclusively with positions at time $t$ denoted as $x_i(t)$. The particles are ordered in such a way that $x_i(t) < x_j(t)$ for $i > j$.
\item Particles jump to the right by one spot ($x_i(t)$ increases by $1$) with jump rate given by $a_i (1-q^{x_{i-1}(t)-x_i(t)+1})$ for $i \ge 2$, where $q \in [0,1)$, $a_i > 0$. The jump rate for the particle $x_1$ is defined to be $a_1$.
\item All jumps occur indenpendently of each other according to exponential clocks with parameter $1$.
\end{itemize}

\begin{figure}
	\centering
	\includegraphics[width=0.5\textwidth]{q-TASEP}
	\caption[An illustration of q-TASEP]
	{An illustration of q-TASEP. The jump rate of the particle $x_2$ is given by $a_2(1-q^2)$, while that of the particle $x_4$ is $0$.}
	\label{fig:q-TASEP}
\end{figure}

It's worth noting that the ordering of the particles remains unchanged throughout the process. Note also that in the definition of q-TASEP, numbering of the particles starts with $1$. However, to facilitate our discussion, we could have added a virtual partical $x_0$ with $x_0 = \infty$ so that the jump rate of $x_1$ is also equal to $a_1 (1-q^{x_0(t) - x_1(t) + 1}) = a_1$. 

It can be easily seen that dynamics of the right most $N$ particles, i.e., particle $x_1$, $x_2$, $\dots$, $x_N$, is independent from those to the left of them, i.e., $x_{N+1}$, $x_{N+2}$, $\dots$ Therefore, from now onwards, we will be focusing on the study of q-TASEP with $N$ particles, with configuration $x_1(t) > x_2(t) > \dots > x_N(t)$. We could then define our state space as $$X^N = \{\vec{x}=(x_0,x_1,\dots, x_N) \in \{\infty \} \times \mathbb{Z}^N : \infty = x_0 > x_1 > \dots > x_N \}.$$

For q-TASEP with $N$ particles, the infinitesimal generator of $\vec{x}(t)$ acting on suitable function $f: X^N \rightarrow \mathbb{R}$, denoted by $L^{q-TASEP} f$, is given by $$(L^{q-TASEP} f) (\vec{x}) = \sum_{i=1}^{N} a_i (1-q^{x_{i-1} - x_i - 1}) (f(\vec{x}_i^{+}) - f(\vec{x})),$$ where $\vec{x}_i^{+}$ denotes the configuration of the q-TASEP with particle $x_i$ jumps to the right by $1$ position, i.e., $\vec{x}_i^+ = (x_0, x_1, \dots, x_{i-1}, x_i+1, x_{i+1}, \dots, x_N)$. This follows from the fact that for $t$ small, there is only $1$ chance for one of the $N$ particles to jump according its own jump rate.

\section{Initial data for q-TASEP}
For a q-TASEP to be well defined, additional to the dynamics of q-TASEP described in Section \ref{sec:intro-qtasep}, we also need an initial configuration of the process, called initial data. In this paper, we focus on two types of initial data, namely, the step initial data and the half stationary initial data. 

Step initial data is defined as the configuration of $x_i(0) = -i$ for $1 \le i \le N$. For half stationary initial data, we define q-Geometric distribution. 

\begin{definition}
\label{def:qgeo}
For $\alpha \in [0,1)$, we say that a random variable $X$ follows the q-Geometric distribution with parameter $\alpha$ [written as $X \sim qGeo(\alpha)$] if $$\mathbb{P}(X = k) = (\alpha;q)_{\infty} \frac{\alpha^k}{(q;q)_k},$$ where $(a;q)_n = (1-a)(1-aq)(1-aq^2)\dots(1-aq^{n-1})$ and $(a;q)_{\infty} = (1-a)(1-aq)(1-aq^2)\dots$
\end{definition}

Let $X_i \sim qGeo(\alpha/a_i)$ for $1 \le i \le N$ be $N$ independent q-Geometric random variables. Then the half stationary initial condition is defined recursively by first setting $x_1(0) = -1 + X_1$ and letting $x_i(0) = -1 + x_{i-1}(0) + X_i$ for $i > 1$. Note that when $\alpha = 0$, the step initial data is recovered.

\section{q-TASEP for a few particles}
The main goal for the study of q-TASEP in this thesis is to identify an exact formula for the distribution of the particle positions, $\mathbb{P}(x_N(t) = m)$ for $m \in \mathbb{Z}$ with step and half stationary initial data. In this section, we provide some intuitions of how this problem can be approached via elementary methods for q-TASEP of $1$ and $2$ particles, thereby illustrating how the complexity grows for $N$ large. 

\subsection{q-TASEP with $1$ particle}
In this section we focus on the q-TASEP with only $1$ particle denoted by $x_1$ starting at position $x_1(0) = 0$. Let $T_i$, $i = 1,2,\dots$ be independent and identically distributed exponential random variables with parameter $1$ denoting the time between the $(i-1)th$ and the $ith$ jump. For $m \in \mathbb{Z}_{\ge 0}$, define $$a_m = \mathbb{P}(x_1(t) \le m) = \mathbb{P}(\sum_{i=1}^{m+1} T_i > t)$$ such that $\mathbb{P}(x_1(t) = m) = a_m - a_{m-1}$ for $m \ge 1$ and $\mathbb{P}(x_1(t) = 0) = a_0 = e^{-t}$. Since $T_i \sim exp(1)$, $\sum_{i=1}^{m} T_i \sim Erlang(m,1)$ and therfore, by the density function of Erlang distribution, $$1 - a_m = \int_0^t \frac{s^m}{m!} e^{-s} ds.$$ 

\begin{proposition}
For q-TASEP with one particle $x_1$ with jump rate parameter $a_1 = 1$ and initial profile at $x_1(0) = -1$, we have that $\mathbb{E}[x_1(t)+1] = t$ and $\mathbb{E}[q^{x_1(t)+1}] = e^{(q-1)t}$.
\end{proposition}

\begin{proof}
From the notations above, we have that $\mathbb{P}(x_1(t) = m) = c_m - c_{m-1}$, where $c_m$ is defined by $c_m = 1 - \int_0^t \frac{s^m}{m!} e^{-s} ds$. Therefore, we have
\begin{align*}
\mathbb{E}[x_1(t)] &=  \lim_{n \to \infty} ((1-c_0) + (1-c_1) + ... + (1-c_{n-1}) - n ( 1-c_n))\\
  						&= \lim_{n \to \infty} (\int_{0}^{t} e^{-s}  (\sum_{i=0}^{n-1} \frac{s^i}{i!}) ds) +\lim_{n \to \infty} (n \times \int_{0}^{t} \frac{s^n}{n!} e^{-s} ds)\\
						&=  \int_{0}^{t} e^{-s} \lim_{n \to \infty} (\sum_{i=0}^{n-1} \frac{s^i}{i!}) ds + 0\\
						&=  \int_{0}^{t} e^{-s} e^s dt\\
						&= t
\end{align*}
Moreover, $\mathbb{E}[q^{x_0(t)}]$ can be computed as below: 
\begin{align*}
\mathbb{E}[q^{x_0(t)}] &= \lim_{n \to \infty} (q^0  c_0 + \sum_{i=1}^{n} q^i (c_i - c_{i-1}) )\\
											 &= \lim_{n \to \infty} (-(1-q) (\sum_{i=0}^{n-1} q^i (1-a_i)) - q^n (1-c_n) + 1)\\
											 &= - (1-q) \lim_{n \to \infty} ( \int_{0}^{t} e^{-s} \sum_{i=0}^{n-1} q^i \frac{s^i}{i!} ds) - \lim_{n \to \infty} \int_0^t q^n \frac{s^n}{n!} ds + 1\\
											 &=  - (1-q) \int_0^t e^{-s }  \lim_{n \to \infty} \sum_{i=0}^{n-1} q^i \frac{s^i}{i!} ds- \lim_{n \to \infty} \int_0^t q^n \frac{s^n}{n!} ds + 1\\
				     					 &=  - (1-q) \int_0^t e^{-s } e^{qs}  ds -\lim_{n \to \infty}  \int_0^t q^n \frac{s^n}{n!} ds + 1\\
				     					 &= e^{(q-1)t}.
\end{align*}
\end{proof}

\subsection{q-TASEP with $2$ particles}
Elementary methods similar to the one adopted for the one-particle system were applied for the $2$ particles system, and it was realized that the computation grew so complicated that nearly no conclusions was reached. Therefore, a different approach, namely the Komogorov Equation, was used to carry out the computation. Although no final conclusion was reached either at the end, some interesting results were found. 

Let us consider the two particles labeled as $x_1$ and $x_2$ starting at the initial positions that $x_1(0) = 0$ and $x_2(0) = a << 0$. Let $\mathbb{P}_{k,j}(t) = \mathbb{P}(x_1(t) = k, x_2(t) = j)$. We begin by giving the Komogorov Equation for the problem:
$$\frac{d}{dt} \mathbb{P}_{k,j}(t) = - \mathbb{P}_{k,j}(t) - (1-q^{k-j-1})\mathbb{P}_{k,j}(t) + (1-q^{k-j})\mathbb{P}_{k,j-1}(t) + \mathbb{P}_{k-1,j}(t)$$
with base cases  $\mathbb{P}_{k,j}(t) = 0$ if $j < a$ or $k < 0$ or $j \ge k$.\\
We will be applying induction on $k$ and $j$ separately, starting by iterating through $k = 0, 1, 2, \dots$. The result is stated as a proposition.
\begin{proposition}
With the notations and setting introduced above, for $m \ge 1$
 $$ \mathbb{P}_{m,a}(t) =\frac{1}{2 \pi i} \oint_{all poles} \frac{e^{(-2+z)t}}{(z-q^{-a-1})(z-q^{-a})...(z-q^{-a+m-1})} dz.$$
\end{proposition}
\begin{proof}
We will not be showing a complete proof here. Rather, we give some calculations for some base cases to check that the proposition is correct and provide some intuitions. \\
\textbf{Case 1}: For $k=0,j=a<0$, we have $$\frac{d}{dt} \mathbb{P}_{0,a}(t) + (2-q^{-a-1}) \mathbb{P}_{0,a}(t) = 0$$
 Solving this equation gives $$\mathbb{P}_{0,a}(t) = c e^{-(2-q^{-a-1})t}$$
 Notice that $\mathbb{P}_{0,a}(0) = 1$, then $c=1$. Therefore $$\mathbb{P}_{0,a}(t) = e^{-(2-q^{-a-1})t} = \frac{1}{2 \pi i} \oint_{all poles} \frac{e^{(-2+z)t}}{z-q^{-a-1}} dz$$
 \textbf{Case 2}: For $k=1, j=a<0$, we have $$\frac{d}{dt} \mathbb{P}_{1,a}(t) + (2-q^{-a}) \mathbb{P}_{1,a}(t) = e^{-(2-q^{-a-1})t}$$
 Therefore, $$\frac{d}{dt} [e^{(2-q^{-a})t} \mathbb{P}_{1,a}(t)] = e^{(q^{-a-1} - q^{-a})t}$$
 Solving this equation we have $$ \mathbb{P}_{1,a}(t) = \frac{e^{-(2-q^{-a-1})t}}{q^{-a-1} - q^{-a}} + c e^{-(2-q^{-a})t}$$
 Note that $\mathbb{P}_{1,a}(0) = 0$, we have $c = -\frac{1}{q^{-a-1} - q^{-a}}$ and therefore $$\mathbb{P}_{1,a}(t) = \frac{1}{q^{-a-1} - q^{-a}} (e^{-(2-q^{-a-1})t} - e^{-(2-q^{-a})t})$$
 In \textbf{contour integral} form, it can also be written as $$\mathbb{P}_{1,a}(t) =\frac{1}{2 \pi i} \oint_{all poles} \frac{e^{(-2+z)t}}{(z-q^{-a-1})(z-q^{-a})} dz$$
 \textbf{Case 3}: For $k=2, j=a<0$, we have $$\frac{d}{dt} \mathbb{P}_{2,a}(t) + (2-q^{1-a}) \mathbb{P}_{2,a}(t) = \mathbb{P}_{1,a}(t)$$
 Solving this equation gives 

 \begin{align*}
  \mathbb{P}_{2,a}(t) &= \frac{e^{(-2+q^{-a-1})t}}{ (q^{-a-1} - q^{-a})(q^{-a-1} - q^{1-a}) } - \frac{ e^{(-2+q^{-a})t} }{ (q^{-a-1} - q^{-a}) (q^{-a} - q^{1-a}) }\\
  & \quad + \frac{e^{(-2+q^{-a+1})t}}{ (q^{-a-1} - q^{-a+1})(q^{-a} - q^{-a+1}) } \\
  &=\frac{1}{2 \pi i} \oint_{all poles} \frac{e^{(-2+z)t}}{(z-q^{-a-1})(z-q^{-a})(z-q^{-a+1})} dz
 \end{align*}
\end{proof}
Next, we investigate the cases $k = 0, j = a, (a+1), \dots, -1$. The result is stated as the following proposition.
\begin{proposition}
With the notations and setting introduced above, for $k = 0, j = a+n$, $0 \le n < a$, we have \\
\begin{align*}
\mathbb{P}_{0,a+n} (t) &= \frac{(1-q^{-a-1})(1-q^{-a-2})...(1-q^{-a-n})}{2 \pi i} \\
& \quad \times \oint_{all poles} \frac{e^{(-2+z)t}}{(z-q^{-a-1})(z-q^{-a-2})...(z-q^{-a-n-1})} dz.
\end{align*}
\end{proposition}

\begin{proof}
Again, we will only be providing some intuitions regarding the equality. \\
For $k=0, j=a+1$, we have $$\frac{d}{dt} \mathbb{P}_{0,a+1}(t) + (2-q^{-a-2}) \mathbb{P}_{0,a+1}(t) = (1-q^{-a-1}) \mathbb{P}_{0,a}(t)$$
 Solving this equation gives 

 \begin{align*}
 \mathbb{P}_{0,a+1} (t) &= \frac{1-q^{-a-1}}{q^{-a-1} - q^{-a-2}} (e^{-(2-q^{-a-1})t} - e^{-(2-q^{-a-2})t})\\
 &= (1-q^{-a-1}) \frac{1}{2 \pi i} \oint_{all poles} \frac{e^{(-2+z)t}}{(z-q^{-a-1})(z-q^{-a-2})} dz
 \end{align*}
\end{proof}

More general application of induction on both $k$ and $j$ together was carried out and didn't reach any elegant results as the ones mentioned above. Therefore, the elementary calculation for the q-TASEP model was stopped and the focus was then turned to studying the duality approach. However, such calculations demonstrate how fast the complexity grows with the number of particles considered, and they were also important as they provided essential fundamental understanding of the model. 

\section{Introduction to q-TAZRP}
Next, we introduce another Markov process called q-TAZRP, short for q-deformed totally asymmetric zero range process. q-TAZRP on an interval $\{0,1,...,N\}$ is a continuous time, discrete space Markov process $\vec{y}(t)$ with state space $$Y^N = (\mathbb{Z}_{\ge 0})^{N+1}$$ subject to the condition of $\sum_{i=0}^{N} y_i(t) = \sum_{i=0}^{N} y_i(0)$ $\forall$ $t\in\mathbb{R}_{\ge 0}$. Dynamics of a q-TAZRP is defined as the following:
\begin{itemize}
\item For each $i \in \{1,2,\dots,N\}$, $y_i(t)$ decreases by $1$ and $y_{i-1}(t)$ increases by $1$ simultaneously according to a rate function given by $g_i(k) = a_i (1-q^{y_i(t)})$.
\item All changes occur independently for each site according to exponential clocks.
\item $y_0$ is always non-decreasing.
\end{itemize}

\begin{figure}
	\centering
	\includegraphics[width=0.75\textwidth]{q-TAZRP}
	\caption[An illustration of q-TAZRP]
	{An illustration of q-TAZRP. Rate function for site $y_1$ is given by $a_1 (1-q^2)$.}
	\label{fig:qTAZRP}
\end{figure}

A natural interpretation of the q-TAZRP is given in Figure \ref{fig:qTAZRP}, where a total of $\sum_{i=0}^{N} y_i(0)$ particles occupy the $N$ sites ordered in such a way that $y_i$ is to the left of $y_{i-1}$ for $i = 1,2,\dots,N$. The changes in the definition then refer to a jump of the top particle at site $y_i$ to the site $y_{i-1}$. Note then that no particle leaves site $0$.

It can be shown that the infinitesimal generator of $\vec{y}(t)$ acting on a suitable function $h:Y^N \rightarrow \mathbb{R}$, denoted as $L^{q-TAZRP} h$, is given by $$(L^{q-TAZRP} h)(\vec{y}) = \sum_{i=1}^{N} a_i (1-q^{y_i}) (h(\vec{y}^{i,i-1}) - h(\vec{y})),$$ where $\vec{y}^{i,i-1}$ represents the configuration of $(y_0, \dots, y_{i-2}, y_{i-1}+1, y_i - 1, y_{i+1}, \dots, y_N)$.

Lastly, we present another notation, $\vec{n} \in W^k_{>0}$, for the states of a q-TAZRP, where $W^k_{>0} = \{(n_1,n_2,\dots,n_k) \in (\mathbb{Z}_{>0})^k : n_1 \ge n_2 \ge \dots \ge n_k \ge 0 \}$. The vector $\vec{n}(\vec{y})$ for any state $\vec{y}$ of the q-TAZRP is given by $$y_i = \left| \{ n_j : n_j = i \} \right|.$$ The intuition is that while $y_i$ in $\vec{y}$ denotes the number of particles at site $i$, $n_j$ in $\vec{n}$ denotes the positioin of Particle $j$ ordered according to decreasing site locations. Take the configuration in Figure \ref{fig:qTAZRP} for example. Its representation in $\vec{y}$ is given by $\vec{y} = (1,2,0,1,0,1,2)$, while in $\vec{n}$ it is represented as $\vec{n} = (6,6,5,3,1,1,0)$. 
